fairness/lawyer/examples/rt_bound/rt_bound.v
@@ -5,37 +5,19 @@ From trillium.fairness Require Import utils.
 From trillium.fairness.lawyer.examples Require Import obls_tactics.
 From trillium.fairness.lawyer.examples.nondet Require Import nondet.
 From trillium.fairness.lawyer.examples.const_term Require Import const_term.
-From trillium.fairness.lawyer.obligations Require Import obligations_model obligations_resources obligations_am obligations_em obligations_logic.
+From trillium.fairness.lawyer.obligations Require Import obligations_model obligations_resources obligations_am obligations_em obligations_logic env_helpers.
 From trillium.fairness.lawyer Require Import sub_action_em program_logic.
 From iris.algebra Require Import auth gmap gset excl excl_auth csum mono_nat.
 From iris.base_logic.lib Require Import invariants.
 
 
 Section RTBound.
-  Context `{ODd: OfeDiscrete DegO} `{ODl: OfeDiscrete LevelO}.
-  Context `{LEl: @LeibnizEquiv (ofe_car LevelO) (ofe_equiv LevelO)}.
-  
-  Let Degree := ofe_car DegO.
-  Let Level := ofe_car LevelO.
-
-  Context `{OPRE: ObligationsParamsPre Degree Level LIM_STEPS}.
-  Let OP := LocaleOP (Locale := locale heap_lang).
-  Existing Instance OP.
-  Let OM := ObligationsModel.
-  
-  Let OAM := ObligationsAM.
-  Let ASEM := ObligationsASEM.
-
+  Context {DegO LvlO LIM_STEPS} {OP: OP_HL DegO LvlO LIM_STEPS}.
   Context `{EM: ExecutionModel heap_lang M}.
+  Notation "'Degree'" := (om_hl_Degree). 
+  Notation "'Level'" := (om_hl_Level).  
 
-  Context {Σ: gFunctors}.
-  (* Keeping the more general interface for future developments *)
-  Context `{oGS': @asem_GS _ _ ASEM Σ}.
-  Let oGS: ObligationsGS (OP := OP) Σ := oGS'.
-  Existing Instance oGS.
-
-  Context `{hGS: @heapGS Σ _ EM}.
-  Let eGS: em_GS Σ := heap_fairnessGS (heapGS := hGS).
+  Context {Σ} {OHE: OM_HL_Env OP EM Σ}. 
 
   Definition rt_bound: val :=
     λ: <>,
@@ -48,8 +30,6 @@ Section RTBound.
   Context (d0 d1: Degree).
   Hypotheses (DEG01: deg_lt d0 d1). 
 
-  Context {OBLS_AMU: @AMU_lift_MU _ _ _ oGS' _ EM _ (↑ nroot)}.
-  Context {OBLS_AMU__f: forall τ, @AMU_lift_MU__f _ _ _ τ oGS' _ EM _ ⊤}.
   Context {NO_OBS_POST: ∀ τ v, obls τ ∅ -∗ fork_post τ v}.
 
   Hypothesis (ND_LB_LS: nondet_LS_LB <= LIM_STEPS).
@@ -77,7 +57,7 @@ Section RTBound.
     { exact l__f. }
     { apply DEG01. }
     { apply DIL_LS. }
-    1-4: by eauto.
+    1-2: by eauto.
     iIntros "!> %v (%n & %π' & -> & #EBn & OB & PH & %PH_LE)".
     rewrite cp_mul_weaken; [| apply PH_LE| reflexivity].
 
@@ -108,8 +88,6 @@ Section RTBound.
     iApply (decr_spec with "[$PH $DECR_INV $CNT CPSd]").
     { iApply (cp_mul_weaken with "[$]"); [done| ].
       rewrite /DECR_ITER_LEN. lia. }
-    Unshelve.
-    2: { apply OBLS_AMU. } 
     iIntros "!> % _". by iApply "POST".
   Qed.
 
