fairness/lawyer/obligations/obligations_em.v
@@ -222,5 +222,5 @@ Section ObligationsEM.
       asem_valid_evolution_step := obls_ves_wrapper;
       asem_initialization := obls_resources_init;
     |}.
-
+       
 End ObligationsEM.
